tuned state display

src/HOL/IMP/Collecting_Examples.thy
@@ -7,12 +7,19 @@ declare insert_code[code del] union_coset_filter[code del]
 lemma insert_code [code]:  "insert x (set xs) = set (x#xs)"
 by simp
 
+text{* In order to display commands annotated with state sets,
+states must be translated into a printable format as lists of pairs,
+for a given set of variable names. This is what @{text show_acom} does: *}
+
+definition show_acom ::
+  "vname list \<Rightarrow> state set acom \<Rightarrow> (vname*val)list set acom" where
+"show_acom xs = map_acom (\<lambda>S. (\<lambda>s. map (\<lambda>x. (x, s x)) xs) ` S)"
+
+
 text{* The example: *}
 definition "c = WHILE Less (V ''x'') (N 3)
                 DO ''x'' ::= Plus (V ''x'') (N 2)"
 definition C0 :: "state set acom" where "C0 = anno {} c"
-
-definition "show_acom xs = map_acom (\<lambda>S. (\<lambda>s. [(x,s x). x \<leftarrow> xs]) ` S)"
 
 text{* Collecting semantics: *}
 
